about to dive into same_com_help

semantics/proofs_new.v
@@ -41,6 +41,16 @@ Inductive all_diff_in_fw: nvmem -> vmem -> command -> nvmem -> Prop :=
 ( forall(l: loc ), ((getmap N1) l <> (getmap N1c) l) -> (l \in getfstwt W))
 -> all_diff_in_fw N1 V1 c1 N1c.
 
+Inductive all_diff_in_fww: nvmem -> vmem -> command -> nvmem -> Prop :=
+  Diff_in_FWw: forall{N1 V1 c1 N2 V2 c2 N1c O W} (T: trace_cs (N1, V1, c1) (N2, V2, c2) O W),
+    checkpoint \notin O -> (*c2 is nearest checkpoint or termination*)
+  (*  (getdomain N1) = (getdomain N1c) -> alternatively
+                                       could check N2 domain as well instead of this
+ not even clear why i need the domains                                    
+   *)
+( forall(l: loc ), ((getmap N1) l <> (getmap N1c) l) -> (l \in getfstwt W))
+-> all_diff_in_fww N1 V1 c1 N1c.
+
     Lemma agreeonread_ins: forall{N Nend N2: nvmem} {V Vend: vmem}
                         {l: instruction} {crem c1: command}
                    {O : obseq} {W: the_write_stuff},
@@ -382,7 +392,7 @@ Qed.
   exists (Nend2: nvmem), cceval_w (N, V, c) O2 (Nend2, Vend, cend) W2.
 Admitted.
 
-Lemma war_works {N0 N Nend: nvmem} {V Vend: vmem} {c cend: command} {O: obseq} {W: the_write_stuff}
+Lemma war_works1 {N0 N Nend: nvmem} {V Vend: vmem} {c cend: command} {O: obseq} {W: the_write_stuff}
       {Wstart Rstart: warvars}:
     trace_cs (N, V, c) (Nend, Vend, cend) O W ->
     WARok (getdomain N0) Wstart Rstart c ->
@@ -396,6 +406,22 @@ Lemma war_works {N0 N Nend: nvmem} {V Vend: vmem} {c cend: command} {O: obseq} {
           l \in (getdomain N0) \/ l \in Wstart).
   Admitted.
 
+Lemma war_works {N0 N Nend: nvmem} {V Vend: vmem} {c cend: command} {O: obseq} {W: the_write_stuff}:
+    trace_cs (N, V, c) (Nend, Vend, cend) O W ->
+  subset_nvm N0 N ->
+    WARok (getdomain N0) [::] [::] c ->
+    checkpoint \notin O ->
+    all_diff_in_fww N V c (N0 U! Nend).
+  Admitted.
+
+
+Lemma same_com_help {N N1 V c Nend1 Vend cend O W}:
+  all_diff_in_fww N V c N1 ->
+  trace_cs (N1, V, c) (Nend1, Vend, cend) O W ->
+  checkpoint \notin O ->
+  exists (Nend2: nvmem), trace_cs (N, V, c) (Nend2, Vend, cend) O W.
+  Admitted.
+
 Lemma same_com {N0 N V c Nmid Vmid cmid O1 W1 Nend1 Vend cend O2 W2}:
   WARok (getdomain N0) [::] [::] c ->
   subset_nvm N0 N ->
@@ -405,29 +431,9 @@ Lemma same_com {N0 N V c Nmid Vmid cmid O1 W1 Nend1 Vend cend O2 W2}:
   trace_cs (N0 U! Nmid, V, c) (Nend1, Vend, cend) O2 W2 ->
   checkpoint \notin O2 ->
   exists (Nend2: nvmem), trace_cs (N, V, c) (Nend2, Vend, cend) O2 W2.
-  intros.
-  move: (war_works H1 H H2) => Hbwar.
-  rewrite remove_empty in Hbwar.
-  suffices:(
-forall l : loc,
-          l \notin getfstwt W1 ->
-          l \in getwt W1 ->
-          l \in getdomain N0
-            ).
-  intros Hbwarc.
-  move: Vmid cmid N W1 O1 H1 H2 H0 Hbwar Hbwarc H31. clear H.
-  dependent induction H3; intros Vmid cmid N W500 O500 Tmid Ho1 Hsub Hbwar Hbwarc.
-  + exists N. apply (CsTrace_Empty (N, Vend, cend)) .
-  + move: (same_com_c Hsub Tmid Hbwarc H Ho1 H4) => [Nend2 Hend2].
-    exists Nend2. by apply CsTrace_Single.
-  + destruct Cmid as [ [N2 V2] c2].
-    rewrite mem_cat in H4. move/ norP : H4 => [Hcp1 Hcp2].
-    move: (same_com_c Hsub Tmid Hbwarc H0 Ho1 Hcp1) => [Nend2 Hend2].
-    suffices:
-      (exists Nend3, trace_cs (Nend2, V2, c2) (Nend3, Vend, cend) O2 W2).
-    move => [Nend3 Tend].
-    exists Nend3. eapply CsTrace_Cons; try apply Tend; try assumption.
-    eapply IHtrace_cs.
+  intros Hwar Hsub Tmid Ho1 T2 Ho2.
+  move: (war_works Tmid Hsub Hwar Ho1) => Hdiff.
+  eapply same_com_help; try apply Hdiff; try assumption. apply T2.
   Admitted. 
 
 Lemma same_comi {N0 N V c O1 W1 Nend Vend cend }:
